Test/og/multiset.bpl
@@ -4,10 +4,10 @@ const unique null : int;
 const unique nil: X;
 const unique done: X;
 
-var {:qed} elt : [int]int;
-var {:qed} valid : [int]bool;
-var {:qed} lock : [int]X;
-var {:qed} owner : [int]X;
+var elt : [int]int;
+var valid : [int]bool;
+var lock : [int]X;
+var owner : [int]X;
 const max : int;
 
 function {:builtin "MapConst"} MapConstBool(bool) : [X]bool;
@@ -18,8 +18,8 @@ function {:inline} {:linear "tid"} TidCollector(x: X) : [X]bool
 
 axiom (max > 0);
 
-procedure {:yields} acquire(i : int, {:linear "tid"} tidIn: X) returns ({:linear "tid"} tidOut: X);
-ensures {:right 0} |{ A: 
+procedure {:yields} {:phase 0} acquire(i : int, {:linear "tid"} tidIn: X) returns ({:linear "tid"} tidOut: X);
+ensures {:right} |{ A: 
                       assert 0 <= i && i < max;
                       assert tidIn != nil && tidIn != done;
                       assume lock[i] == nil;
@@ -29,8 +29,8 @@ ensures {:right 0} |{ A:
                     }|;
 
 
-procedure {:yields} release(i : int, {:linear "tid"} tidIn: X) returns ({:linear "tid"} tidOut: X);
-ensures {:left 0} |{ A: 
+procedure {:yields} {:phase 0} release(i : int, {:linear "tid"} tidIn: X) returns ({:linear "tid"} tidOut: X);
+ensures {:left} |{ A: 
                      assert 0 <= i && i < max;
                      assert lock[i] == tidIn;
                      assert tidIn != nil && tidIn != done; 
@@ -40,8 +40,8 @@ ensures {:left 0} |{ A:
                     }|;
 
 
-procedure {:yields} getElt(j : int, {:linear "tid"} tidIn: X) returns ({:linear "tid"} tidOut: X, elt_j:int);
-ensures {:both 0,1} |{ A: 
+procedure {:yields} {:phase 0,1} getElt(j : int, {:linear "tid"} tidIn: X) returns ({:linear "tid"} tidOut: X, elt_j:int);
+ensures {:both} |{ A: 
                      assert 0 <= j && j < max;
                      assert lock[j] == tidIn;
                      assert tidIn != nil && tidIn != done;
@@ -51,8 +51,8 @@ ensures {:both 0,1} |{ A:
                     }|;
 
 
-procedure {:yields} setElt(j : int, x : int, {:linear "tid"} tidIn: X) returns ({:linear "tid"} tidOut: X);
-ensures {:both 0,1} |{ A: 
+procedure {:yields} {:phase 0,1} setElt(j : int, x : int, {:linear "tid"} tidIn: X) returns ({:linear "tid"} tidOut: X);
+ensures {:both} |{ A: 
                      assert x != null;
                      assert owner[j] == nil;
                      assert 0 <= j && j < max;
@@ -65,8 +65,8 @@ ensures {:both 0,1} |{ A:
                     }|;
 
 
-procedure {:yields} setEltToNull(j : int, {:linear "tid"} tidIn: X) returns ({:linear "tid"} tidOut: X);
-ensures {:left 0} |{ A: 
+procedure {:yields} {:phase 0} setEltToNull(j : int, {:linear "tid"} tidIn: X) returns ({:linear "tid"} tidOut: X);
+ensures {:left} |{ A: 
                      assert owner[j] == tidIn;
                      assert 0 <= j && j < max;
                      assert lock[j] == tidIn;
@@ -78,8 +78,8 @@ ensures {:left 0} |{ A:
                      return true;
                     }|;
 
-procedure {:yields} setValid(j : int, {:linear "tid"} tidIn: X) returns ({:linear "tid"} tidOut: X);
-ensures {:both 0} |{ A: 
+procedure {:yields} {:phase 0} setValid(j : int, {:linear "tid"} tidIn: X) returns ({:linear "tid"} tidOut: X);
+ensures {:both} |{ A: 
                      assert 0 <= j && j < max;
                      assert lock[j] == tidIn;
                      assert tidIn != nil && tidIn != done;
@@ -90,8 +90,8 @@ ensures {:both 0} |{ A:
                      return true;
                     }|;
 
-procedure {:yields} isEltThereAndValid(j : int, x : int, {:linear "tid"} tidIn: X) returns ({:linear "tid"} tidOut: X, fnd:bool);
-ensures {:both 0} |{ A: 
+procedure {:yields} {:phase 0} isEltThereAndValid(j : int, x : int, {:linear "tid"} tidIn: X) returns ({:linear "tid"} tidOut: X, fnd:bool);
+ensures {:both} |{ A: 
                        assert 0 <= j && j < max;
                        assert lock[j] == tidIn;
                        assert tidIn != nil && tidIn != done;
@@ -100,10 +100,10 @@ ensures {:both 0} |{ A:
                        return true;
                     }|;
 
-procedure {:yields} FindSlot(x : int, {:linear "tid"} tidIn: X) returns (r : int, {:linear "tid"} tidOut: X)
+procedure {:yields} {:phase 1} FindSlot(x : int, {:linear "tid"} tidIn: X) returns (r : int, {:linear "tid"} tidOut: X)
 requires {:phase 1} Inv(valid, elt, owner);
 ensures {:phase 1} Inv(valid, elt, owner);
-ensures {:right 1}  |{ A: assert tidIn != nil && tidIn != done; 
+ensures {:right}  |{ A: assert tidIn != nil && tidIn != done; 
                           assert x != null; 
 			  goto B, C;
                        B: assume (0 <= r && r < max); 
@@ -159,12 +159,12 @@ ensures {:right 1}  |{ A: assert tidIn != nil && tidIn != done;
 	return;
 }
 
-procedure {:yields} Insert(x : int, {:linear "tid"} tidIn: X) returns (result : bool, {:linear "tid"} tidOut: X) 
+procedure {:yields} {:phase 2} Insert(x : int, {:linear "tid"} tidIn: X) returns (result : bool, {:linear "tid"} tidOut: X) 
 requires {:phase 1} Inv(valid, elt, owner);
 requires {:phase 2} Inv(valid, elt, owner);
 ensures {:phase 1} Inv(valid, elt, owner);
 requires {:phase 2} Inv(valid, elt, owner);
-ensures {:atomic 2}  |{ var r:int;
+ensures {:atomic}  |{ var r:int;
                         A: assert tidIn != nil && tidIn != done; 
                            assert x != null;
                            goto B, C;
@@ -204,7 +204,7 @@ ensures {:atomic 2}  |{ var r:int;
 	return;
 }
 
-procedure {:yields} InsertPair(x : int, 
+procedure {:yields} {:phase 2} InsertPair(x : int, 
                                y : int, 
                                {:linear "tid"} tidIn: X) 
                                returns (result : bool, 
@@ -213,7 +213,7 @@ requires {:phase 1} Inv(valid, elt, owner);
 ensures {:phase 1} Inv(valid, elt, owner);
 requires {:phase 2} Inv(valid, elt, owner);
 ensures {:phase 2} Inv(valid, elt, owner);
-ensures {:atomic 2}  |{ var rx:int;
+ensures {:atomic}  |{ var rx:int;
                         var ry:int;
                         A: assert tidIn != nil && tidIn != done; 
                            assert x != null && y != null;
@@ -285,12 +285,12 @@ ensures {:atomic 2}  |{ var rx:int;
 	return;
 }
 
-procedure {:yields} LookUp(x : int, {:linear "tid"} tidIn: X, old_valid:[int]bool, old_elt:[int]int) returns (found : bool, {:linear "tid"} tidOut: X)
+procedure {:yields} {:phase 2} LookUp(x : int, {:linear "tid"} tidIn: X, old_valid:[int]bool, old_elt:[int]int) returns (found : bool, {:linear "tid"} tidOut: X)
 requires {:phase 1} {:phase 2} old_valid == valid && old_elt == elt;
 requires {:phase 1} {:phase 2} Inv(valid, elt, owner);
 requires {:phase 1} {:phase 2} (tidIn != nil && tidIn != done);
 ensures {:phase 1} {:phase 2} Inv(valid, elt, owner);
-ensures {:atomic 2}  |{ A: assert tidIn != nil && tidIn != done; 
+ensures {:atomic}  |{ A: assert tidIn != nil && tidIn != done; 
                           assert x != null;
                           assume found ==> (exists ii:int :: 0 <= ii && ii < max && valid[ii] && elt[ii] == x);
 			  assume !found ==> (forall ii:int :: 0 <= ii && ii < max ==> !(old_valid[ii] && old_elt[ii] == x));
@@ -335,14 +335,13 @@ ensures {:atomic 2}  |{ A: assert tidIn != nil && tidIn != done;
 	return;
 }
 
-procedure {:yields} {:stable} Yield1()
+procedure {:yields} {:phase 1} Yield1()
 requires {:phase 1} Inv(valid, elt, owner);
 ensures {:phase 1} Inv(valid, elt, owner);
-ensures {:both 1} |{ A: return true; }|;
 {
 }
 
-procedure {:yields} {:stable} Yield12()
+procedure {:yields} {:phase 2} Yield12()
 requires {:phase 1} {:phase 2} Inv(valid, elt, owner);
 ensures {:phase 1} {:phase 2} Inv(valid, elt, owner);
 {
@@ -355,7 +354,7 @@ function {:inline} Inv(valid: [int]bool, elt: [int]int, owner: [int]X): (bool)
    (forall i:int :: 0 <= i && i < max ==> (elt[i] == null <==> (!valid[i] && owner[i] == nil)))
 }
 
-procedure {:yields} {:stable} YieldLookUp(old_valid: [int]bool, old_elt: [int]int)
+procedure {:yields} {:phase 2} YieldLookUp(old_valid: [int]bool, old_elt: [int]int)
 requires {:phase 1} {:phase 2} (forall ii:int :: 0 <= ii && ii < max && old_valid[ii] ==> valid[ii] && old_elt[ii] == elt[ii]);
 ensures {:phase 1} {:phase 2} (forall ii:int :: 0 <= ii && ii < max && old_valid[ii] ==> valid[ii] && old_elt[ii] == elt[ii]);
 {
