Test/og/ticket.bpl
@@ -6,10 +6,10 @@ axiom (forall x: int, y: int :: RightClosed(x)[y] <==> y <= x);
 type X;
 function {:builtin "MapConst"} mapconstbool(bool): [X]bool;
 const nil: X;
-var {:qed} t: int;
-var {:qed} s: int;
-var {:qed} cs: X;
-var {:qed} T: [int]bool;
+var {:phase 3} t: int;
+var {:phase 3} s: int;
+var {:phase 3} cs: X;
+var {:phase 3} T: [int]bool;
 
 function {:builtin "MapConst"} MapConstBool(bool) : [X]bool;
 function {:inline} {:linear "tid"} TidCollector(x: X) : [X]bool
@@ -34,7 +34,7 @@ function {:inline} Inv2(tickets: [int]bool, ticket: int, lock: X): (bool)
 procedure Allocate({:linear "tid"} xls':[X]bool) returns ({:linear "tid"} xls: [X]bool, {:linear "tid"} xl: X);
 ensures {:phase 1} {:phase 2} xl != nil;
 
-procedure {:yields} {:entrypoint} main({:linear "tid"} xls':[X]bool)
+procedure {:yields} {:phase 3} main({:linear "tid"} xls':[X]bool)
 requires {:phase 3} xls' == mapconstbool(true);
 {
     var {:linear "tid"} tid: X;
@@ -50,12 +50,15 @@ requires {:phase 3} xls' == mapconstbool(true);
     invariant {:phase 1} Inv1(T, t);
     invariant {:phase 2} Inv2(T, s, cs);
     {
+	par Yield1() | Yield2() | Yield();
         call xls, tid := Allocate(xls);
         async call Customer(tid);
+    	par Yield1() | Yield2() | Yield();
+
     }
 }
 
-procedure {:yields} {:stable} Customer({:linear "tid"} tid': X)
+procedure {:yields} {:phase 3} Customer({:linear "tid"} tid': X)
 requires {:phase 1} Inv1(T, t);
 requires {:phase 2} tid' != nil && Inv2(T, s, cs);
 requires {:phase 3} true;
@@ -75,12 +78,12 @@ requires {:phase 3} true;
     }
 }
 
-procedure {:yields} Enter({:linear "tid"} tid': X) returns ({:linear "tid"} tid: X)
+procedure {:yields} {:phase 2,3} Enter({:linear "tid"} tid': X) returns ({:linear "tid"} tid: X)
 requires {:phase 1} Inv1(T, t);
 ensures {:phase 1} Inv1(T,t);
 requires {:phase 2} tid' != nil && Inv2(T, s, cs);
 ensures {:phase 2} tid != nil && Inv2(T, s, cs);
-ensures {:right 2} |{ A: tid := tid'; havoc t, T; assume tid != nil && cs == nil; cs := tid; return true; }|;
+ensures {:right} |{ A: tid := tid'; havoc t, T; assume tid != nil && cs == nil; cs := tid; return true; }|;
 {
     var m: int;
 
@@ -92,10 +95,10 @@ ensures {:right 2} |{ A: tid := tid'; havoc t, T; assume tid != nil && cs == nil
     par Yield1() | Yield2();
 }
 
-procedure {:yields} GetTicketAbstract({:linear "tid"} tid': X) returns ({:linear "tid"} tid: X, m: int)
+procedure {:yields} {:phase 1,2} GetTicketAbstract({:linear "tid"} tid': X) returns ({:linear "tid"} tid: X, m: int)
 requires {:phase 1} Inv1(T, t);
 ensures {:phase 1} Inv1(T, t);
-ensures {:right 1,2} |{ A: tid := tid'; havoc m, t; assume !T[m]; T[m] := true; return true; }|;
+ensures {:right} |{ A: tid := tid'; havoc m, t; assume !T[m]; T[m] := true; return true; }|;
 {
     par Yield1();
     tid := tid';
@@ -103,33 +106,31 @@ ensures {:right 1,2} |{ A: tid := tid'; havoc m, t; assume !T[m]; T[m] := true; 
     par Yield1();
 }
 
-procedure {:yields} {:stable} Yield()
+procedure {:yields} {:phase 3} Yield()
 {
 }
 
-procedure {:yields} {:stable} Yield2()
+procedure {:yields} {:phase 2} Yield2()
 requires {:phase 2} Inv2(T, s, cs);
 ensures {:phase 2} Inv2(T, s, cs);
-ensures {:both 2} |{ A: return true; }|;
 {
 }
 
-procedure {:yields} {:stable} Yield1()
+procedure {:yields} {:phase 1} Yield1()
 requires {:phase 1} Inv1(T, t);
 ensures {:phase 1} Inv1(T,t);
-ensures {:both 1} |{ A: return true; }|;
 {
 }
 
-procedure {:yields} Init({:linear "tid"} xls':[X]bool) returns ({:linear "tid"} xls:[X]bool);
-ensures {:atomic 0} |{ A: assert xls' == mapconstbool(true); xls := xls'; cs := nil; t := 0; s := 0; T := RightOpen(0); return true; }|;
+procedure {:yields} {:phase 0,3} Init({:linear "tid"} xls':[X]bool) returns ({:linear "tid"} xls:[X]bool);
+ensures {:atomic} |{ A: assert xls' == mapconstbool(true); xls := xls'; cs := nil; t := 0; s := 0; T := RightOpen(0); return true; }|;
 
-procedure {:yields} GetTicket({:linear "tid"} tid': X) returns ({:linear "tid"} tid: X, m: int);
-ensures {:atomic 0,1} |{ A: tid := tid'; m := t; t := t + 1; T[m] := true; return true; }|;
+procedure {:yields} {:phase 0,1} GetTicket({:linear "tid"} tid': X) returns ({:linear "tid"} tid: X, m: int);
+ensures {:atomic} |{ A: tid := tid'; m := t; t := t + 1; T[m] := true; return true; }|;
 
-procedure {:yields} WaitAndEnter({:linear "tid"} tid': X, m:int) returns ({:linear "tid"} tid: X);
-ensures {:atomic 0,2} |{ A: tid := tid'; assume m <= s; cs := tid; return true; }|;
+procedure {:yields} {:phase 0,2} WaitAndEnter({:linear "tid"} tid': X, m:int) returns ({:linear "tid"} tid: X);
+ensures {:atomic} |{ A: tid := tid'; assume m <= s; cs := tid; return true; }|;
 
-procedure {:yields} Leave({:linear "tid"} tid': X) returns ({:linear "tid"} tid: X);
-ensures {:atomic 0} |{ A: assert cs == tid'; assert tid' != nil; tid := tid'; s := s + 1; cs := nil; return true; }|;
+procedure {:yields} {:phase 0,3} Leave({:linear "tid"} tid': X) returns ({:linear "tid"} tid: X);
+ensures {:atomic} |{ A: assert cs == tid'; assert tid' != nil; tid := tid'; s := s + 1; cs := nil; return true; }|;
 
