Test/og/akash.bpl
@@ -17,18 +17,24 @@ function {:inline} {:linear "2"} SetCollector2(x: [int]bool) : [int]bool
 }
 
 procedure Allocate() returns ({:linear "tid"} xls: int);
-ensures xls != 0;
+ensures {:phase 1} xls != 0;
 
 procedure Allocate_1() returns ({:linear "1"} xls: [int]bool);
-ensures xls == mapconstbool(true);
+ensures {:phase 1} xls == mapconstbool(true);
 
 procedure Allocate_2() returns ({:linear "2"} xls: [int]bool);
-ensures xls == mapconstbool(true);
+ensures {:phase 1} xls == mapconstbool(true);
 
-var g: int;
-var h: int;
+var {:phase 1} g: int;
+var {:phase 1} h: int;
 
-procedure {:yields} A({:linear "tid"} tid_in: int) returns ({:linear "tid"} tid_out: int) 
+procedure {:yields} {:phase 0,1} SetG(val:int);
+ensures {:atomic} |{A: g := val; return true; }|;
+
+procedure {:yields} {:phase 0,1} SetH(val:int);
+ensures {:atomic} |{A: h := val; return true; }|;
+
+procedure {:yields} {:phase 1} A({:linear "tid"} tid_in: int) returns ({:linear "tid"} tid_out: int) 
 {
     var {:linear "1"} x: [int]bool;
     var {:linear "2"} y: [int]bool;
@@ -37,51 +43,62 @@ procedure {:yields} A({:linear "tid"} tid_in: int) returns ({:linear "tid"} tid_
     call x := Allocate_1();
     call y := Allocate_2();
 
-    g := 0;
     yield;
-    assert g == 0 && x == mapconstbool(true);    
+    call SetG(0);
+    yield;
+    assert {:phase 1} g == 0 && x == mapconstbool(true);    
 
     yield;
     call tid_child := Allocate();
     async call B(tid_child, x);
 
     yield;
-    h := 0;
+    call SetH(0);
 
     yield;
-    assert h == 0 && y == mapconstbool(true);    
+    assert {:phase 1} h == 0 && y == mapconstbool(true);    
 
     yield;
     call tid_child := Allocate();
     async call C(tid_child, y);
+
+    yield;
 }
 
-procedure {:yields} {:stable} B({:linear "tid"} tid_in: int, {:linear "1"} x_in: [int]bool) 
-requires x_in != mapconstbool(false);
+procedure {:yields} {:phase 1} B({:linear "tid"} tid_in: int, {:linear "1"} x_in: [int]bool) 
+requires {:phase 1} x_in != mapconstbool(false);
 {
     var {:linear "tid"} tid_out: int;
     var {:linear "1"} x: [int]bool;
     tid_out := tid_in;
     x := x_in;    
 
-    g := 1;
+    yield;
+
+    call SetG(1);
 
     yield;
 
-    g := 2;
+    call SetG(2);
+
+    yield;
 }
 
-procedure {:yields} {:stable} C({:linear "tid"} tid_in: int, {:linear "2"} y_in: [int]bool) 
-requires y_in != mapconstbool(false);
+procedure {:yields} {:phase 1} C({:linear "tid"} tid_in: int, {:linear "2"} y_in: [int]bool) 
+requires {:phase 1} y_in != mapconstbool(false);
 {
     var {:linear "tid"} tid_out: int;
     var {:linear "2"} y: [int]bool;
     tid_out := tid_in;
     y := y_in;    
 
-    h := 1;
+    yield;
+
+    call SetH(1);
 
     yield;
 
-    h := 2;
+    call SetH(2);
+
+    yield;
 }
