Test/og/linear-set.bpl
@@ -18,16 +18,26 @@ function {:inline} {:linear "x"} XCollector(xs: [X]bool) : [X]bool
   xs
 }
 
-var x: int;
-var l: [X]bool;
+var {:phase 1} x: int;
+var {:phase 1} l: [X]bool;
 
 procedure Split({:linear "x"} xls: [X]bool) returns ({:linear "x"} xls1: [X]bool, {:linear "x"} xls2: [X]bool);
 ensures xls == MapOr(xls1, xls2) && xls1 != None() && xls2 != None();
 
 procedure Allocate() returns ({:linear "tid"} xls: [X]bool);
 
-procedure {:entrypoint} {:yields} main({:linear "tid"} tidls': [X]bool, {:linear "x"} xls': [X]bool) 
-requires tidls' != None() && xls' == All();
+procedure {:yields} {:phase 0,1} Set(v: int);
+ensures {:atomic} |{A: x := v; return true; }|;
+
+procedure {:yields} {:phase 0,1} Lock(tidls: [X]bool);
+ensures {:atomic} |{A: assume l == None(); l := tidls; return true; }|;
+
+procedure {:yields} {:phase 0,1} Unlock();
+ensures {:atomic} |{A: l := None(); return true; }|;
+
+
+procedure {:yields} {:phase 1} main({:linear "tid"} tidls': [X]bool, {:linear "x"} xls': [X]bool) 
+requires {:phase 1} tidls' != None() && xls' == All();
 {
     var {:linear "tid"} tidls: [X]bool;
     var {:linear "x"} xls: [X]bool;
@@ -37,22 +47,25 @@ requires tidls' != None() && xls' == All();
 
     tidls := tidls';
     xls := xls';
-
-    x := 42;
     yield;
-    assert xls == All();
-    assert x == 42;
+    call Set(42);
+    yield;
+    assert {:phase 1} xls == All();
+    assert {:phase 1} x == 42;
     call xls1, xls2 := Split(xls);
     call lsChild := Allocate();
     assume (lsChild != None());
+    yield;
     async call thread(lsChild, xls1);
     call lsChild := Allocate();
     assume (lsChild != None());
+    yield;
     async call thread(lsChild, xls2);
+    yield;
 }
 
-procedure {:yields} {:stable} thread({:linear "tid"} tidls': [X]bool, {:linear "x"} xls': [X]bool)
-requires tidls' != None() && xls' != None();
+procedure {:yields} {:phase 1} thread({:linear "tid"} tidls': [X]bool, {:linear "x"} xls': [X]bool)
+requires {:phase 1} tidls' != None() && xls' != None();
 {
     var {:linear "x"} xls: [X]bool;
     var {:linear "tid"} tidls: [X]bool;
@@ -60,15 +73,15 @@ requires tidls' != None() && xls' != None();
     tidls := tidls';
     xls := xls';
 
-    assume l == None();
-    l := tidls;
     yield;
-    assert tidls != None() && xls != None();
-    x := 0;
+    call Lock(tidls);
     yield;
-    assert tidls != None() && xls != None();
-    assert x == 0;
+    assert {:phase 1} tidls != None() && xls != None();
+    call Set(0);
     yield;
-    assert tidls != None() && xls != None();
-    l := None();
+    assert {:phase 1} tidls != None() && xls != None();
+    assert {:phase 1} x == 0;
+    assert {:phase 1} tidls != None() && xls != None();
+    call Unlock();
+    yield;
 }
