Test/og/lock2.bpl
@@ -1,14 +1,18 @@
-var {:qed} b: int;
+var {:phase 2} b: int;
 
-procedure {:yields} {:entrypoint} main()
+procedure {:yields} {:phase 2} main()
 {
     while (*)
     {
+        yield;
+
         async call Customer();
+
+        yield;
     }
 }
 
-procedure {:yields} {:stable} Customer()
+procedure {:yields} {:phase 2} Customer()
 {
     while (*) 
     {
@@ -19,13 +23,15 @@ procedure {:yields} {:stable} Customer()
     	yield;
 
     	call Leave();
+
+        yield;
     }
 
     yield;
 }
 
-procedure {:yields} Enter() 
-ensures {:atomic 1} |{ A: assume b == 0; b := 1; return true; }|;
+procedure {:yields} {:phase 1,2} Enter() 
+ensures {:atomic} |{ A: assume b == 0; b := 1; return true; }|;
 {
     var _old, curr: int;
     while (true) { 
@@ -46,15 +52,15 @@ ensures {:atomic 1} |{ A: assume b == 0; b := 1; return true; }|;
     }
 }
 
-procedure {:yields} Read() returns (val: int);
-ensures {:atomic 0} |{ A: val := b; return true; }|;
+procedure {:yields} {:phase 0,2} Read() returns (val: int);
+ensures {:atomic} |{ A: val := b; return true; }|;
 
-procedure {:yields} CAS(prev: int, next: int) returns (_old: int);
-ensures {:atomic 0} |{ 
+procedure {:yields} {:phase 0,2} CAS(prev: int, next: int) returns (_old: int);
+ensures {:atomic} |{ 
 A: _old := b; goto B, C; 
 B: assume _old == prev; b := next; return true; 
 C: assume _old != prev; return true; 
 }|;
 
-procedure {:yields} Leave();
-ensures {:atomic 0} |{ A: b := 0; return true; }|;
+procedure {:yields} {:phase 0,2} Leave();
+ensures {:atomic} |{ A: b := 0; return true; }|;
