Test/og/new1.bpl
@@ -1,6 +1,6 @@
 function {:builtin "MapConst"} mapconstbool(x:bool): [int]bool;
 
-var g:int;
+var {:phase 1} g:int;
 
 function {:inline} {:linear "Perm"} SetCollectorPerm(x: [int]bool) : [int]bool
 {
@@ -11,30 +11,37 @@ procedure Allocate_Perm({:linear "Perm"} Permissions: [int]bool) returns ({:line
 requires Permissions == mapconstbool(true);
 ensures xls == mapconstbool(true);
 
-procedure {:yields} {:stable} PB({:linear "Perm"} permVar_in:[int]bool)
-requires permVar_in[0] && g == 0;
+procedure {:yields} {:phase 1} PB({:linear "Perm"} permVar_in:[int]bool)
+requires {:phase 1} permVar_in[0] && g == 0;
 {
   var {:linear "Perm"} permVar_out: [int]bool;
   permVar_out := permVar_in;
 
   yield;
-  assert permVar_out[0];
-  assert g == 0;
+  assert {:phase 1} permVar_out[0];
+  assert {:phase 1} g == 0;
 
-  g := g + 1;
+  call IncrG();
 
   yield;
-  assert permVar_out[0];
-  assert g == 1;
+  assert {:phase 1} permVar_out[0];
+  assert {:phase 1} g == 1;
 }
 
-procedure{:entrypoint} {:yields} Main({:linear "Perm"} Permissions: [int]bool)
-requires Permissions == mapconstbool(true);
+procedure {:yields} {:phase 1} Main({:linear "Perm"} Permissions: [int]bool)
+requires {:phase 0,1} Permissions == mapconstbool(true);
 {
   var {:linear "Perm"} permVar_out: [int]bool;
 
   call permVar_out := Allocate_Perm(Permissions);
-
-  g := 0;
+  yield;
+  call SetG(0);
   async call PB(permVar_out);
+  yield;
 }
+
+procedure {:yields} {:phase 0,1} SetG(val:int);
+ensures {:atomic} |{A: g := val; return true; }|;
+
+procedure {:yields} {:phase 0,1} IncrG();
+ensures {:atomic} |{A: g := g + 1; return true; }|;
