Test/og/perm.bpl
@@ -1,4 +1,4 @@
-var x: int;
+var {:phase 1} x: int;
 function {:builtin "MapConst"} ch_mapconstbool(x: bool) : [int]bool;
 
 function {:builtin "MapOr"} ch_mapunion(x: [int]bool, y: [int]bool) : [int]bool;
@@ -12,44 +12,44 @@ procedure Split({:linear "Perm"} xls: [int]bool) returns ({:linear "Perm"} xls1:
   ensures xls == ch_mapunion(xls1, xls2) && xls1 != ch_mapconstbool(false) && xls2 != ch_mapconstbool(false);
 
 
-procedure {:entrypoint} {:yields} mainE({:linear "Perm"} permVar_in: [int]bool)
-   free requires permVar_in == ch_mapconstbool(true);
-   free requires permVar_in[0];
-  modifies x;
+procedure {:yields} {:phase 1} mainE({:linear "Perm"} permVar_in: [int]bool)
+   free requires {:phase 1} permVar_in == ch_mapconstbool(true);
+   free requires {:phase 1} permVar_in[0];
+   free requires {:phase 1} x == 0;
 {
     var {:linear "Perm"} permVar_out: [int]bool;
     var {:linear "Perm"} permVarOut2: [int]bool;
 
     permVar_out := permVar_in;
 
-    assume x == 0;
-
     yield;
-    assert x == 0;
-    assert permVar_out[0];
-    assert permVar_out == ch_mapconstbool(true);
+    assert {:phase 1} x == 0;
+    assert {:phase 1} permVar_out[0];
+    assert {:phase 1} permVar_out == ch_mapconstbool(true);
 
     call permVar_out, permVarOut2 := Split(permVar_out);
     async call foo(permVarOut2);
+    yield;
 }
 
-procedure {:yields} {:stable} foo({:linear "Perm"} permVar_in: [int]bool) 
-  free requires permVar_in != ch_mapconstbool(false);
-  free requires permVar_in[1];
-  requires x == 0;
-  modifies x;
+procedure {:yields} {:phase 1} foo({:linear "Perm"} permVar_in: [int]bool) 
+  free requires {:phase 1} permVar_in != ch_mapconstbool(false);
+  free requires {:phase 1} permVar_in[1];
+  requires {:phase 1} x == 0;
 {
   var {:linear "Perm"} permVar_out: [int]bool;
   permVar_out := permVar_in;
   
   yield;
-  assert permVar_out[1];
-  assert x == 0;
+  assert {:phase 1} permVar_out[1];
+  assert {:phase 1} x == 0;
 
-  x := x + 1;
+  call Incr();
 
   yield;
-  assert permVar_out[1];
-  assert x == 1;
+  assert {:phase 1} permVar_out[1];
+  assert {:phase 1} x == 1;
 }
 
+procedure {:yields} {:phase 0,1} Incr();
+ensures {:atomic} |{A: x := x + 1; return true; }|;
