Test/og/runtest.bat
@@ -9,7 +9,7 @@ for %%f in (foo.bpl bar.bpl one.bpl parallel1.bpl) do (
   %BGEXE% %* /nologo /noinfer %%f
 )
 
-for %%f in (linear-set.bpl linear-set2.bpl FlanaganQadeer.bpl DeviceCacheSimplified.bpl parallel2.bpl parallel4.bpl parallel5.bpl akash.bpl t1.bpl new1.bpl perm.bpl async.bpl DeviceCache.bpl ticket.bpl lock.bpl lock2.bpl multiset.bpl civl-paper.bpl) do (
+for %%f in (linear-set.bpl linear-set2.bpl FlanaganQadeer.bpl parallel2.bpl parallel4.bpl parallel5.bpl akash.bpl t1.bpl new1.bpl perm.bpl DeviceCache.bpl ticket.bpl lock.bpl lock2.bpl multiset.bpl civl-paper.bpl) do (
   echo.
   echo -------------------- %%f --------------------
   %BGEXE% %* /nologo /noinfer /typeEncoding:m /useArrayTheory %%f
